update invariants to be duplicable, prove all local operation specs

src/Examples/DistributedCtr/DistCtrImpl_Local.v
@@ -23,9 +23,16 @@ Definition kill_node: val :=
 
 Section proof.
   Context `{!heapG Σ, !spawnG Σ, !lockG Σ, !inG Σ (authR (optionUR (exclR ZO)))}.
+  Definition nodeN : namespace := nroot .@ "node".
 
-  Definition node_val_inv (node: loc) (n : Z) (optv: option Z) (γ : gname): iProp Σ := 
-      ((⌜ optv = None ⌝ ∗ node ↦ NONEV) ∨ (⌜optv = Some n⌝ ∗ node ↦ SOMEV #n)) ∗ own γ (◯ (Excl' n)).
+  Definition node_val_prop (node: loc) (isDead: Prop) (γ : gname): iProp Σ :=
+    ∃ (n: Z), ((⌜isDead⌝ ∧ node ↦ NONEV) ∨ (⌜~isDead⌝ ∧ node ↦ SOMEV #n))%I.
+
+  Definition node_own_inv (node: loc) (n : Z) (γ : gname): iProp Σ :=
+    own γ (◯ (Excl' n))%I.
+
+  Definition node_val_inv (node: loc) (isDead: Prop) (γ : gname): iProp Σ :=
+    inv nodeN (node_val_prop node isDead γ)%I.
 
   Definition node_lock_inv (γ: gname) : iProp Σ :=
     (∃ n, own γ (● (Excl' n)))%I.
@@ -33,9 +40,10 @@ Section proof.
   Lemma alloc_node_spec : 
     {{{ True%I }}}
       alloc_node #()
-      {{{ r1 lk γ γ1 , RET PairV #r1 lk;
-          is_lock LockN γ lk (node_lock_inv γ1) ∗
-          node_val_inv r1 0 (Some 0) γ1
+      {{{ r1 lk γ γ1, RET PairV #r1 lk;
+          is_lock LockN γ lk (node_lock_inv γ1)
+          ∗ node_val_inv r1 false γ1
+          ∗ node_own_inv r1 0 γ1
     }}}.
   Proof.
     iIntros (Φ) "_ HPost".
@@ -49,35 +57,61 @@ Section proof.
     iExists 0; auto.
     iIntros (lk γ) "HIsLk".
     wp_let.
+    iMod (inv_alloc nodeN _ (node_val_prop master false γ1) with "[Hr1]") as "#Hinv".
+    { unfold node_val_prop. iNext. iExists 0. iRight; iSplit; auto. }
+
     wp_pures.
-    iApply "HPost". 
+    iApply "HPost".
     iFrame; auto.
   Qed.
 
   Lemma update_node_some_spec : ∀ (n: Z) γ1 node,
       {{{
            node_lock_inv γ1
-           ∗ node_val_inv node n (Some n) γ1
+          ∗ node_val_inv node false γ1
+          ∗ node_own_inv node n γ1
     }}}
       update_node #node
     {{{ RET #1;
           node_lock_inv γ1
-          ∗ node_val_inv node (n+1) (Some (n+1)) γ1
+          ∗ node_val_inv node false γ1
+          ∗ node_own_inv node (n+1) γ1
     }}}.
   Proof.
-    iIntros (n γ1 node Φ) "(Hlkinv & Hnodeinv) HPost".
+    iIntros (n γ1 node Φ) "(Hlkinv & #Hnodeinv & Hγ1◯) HPost".
     unfold node_val_inv.
-    iDestruct "Hnodeinv" as "([(H & Halive) | (H & Halive)] & Hown)".
-    iDestruct "H" as %H. inversion H. 
+    unfold node_val_prop.
     unfold update_node.
     unfold node_lock_inv.
-    iDestruct "Hlkinv" as (n') "Hlkinv".
-    iMod (ghost_var_update γ1 (n+1) with "Hlkinv Hown") as "[Hγ1● Hγ1◯]".
+    unfold node_own_inv.
     wp_pures.
-    wp_load.
+
+    wp_bind ( ! #node )%E.
+    iInv "Hnodeinv" as ">Hinv".
+    iDestruct "Hinv" as (n') "[[H Halive] | [H Halive]]";
+    wp_load;
+    iDestruct "H" as %H. inversion H.
+    iModIntro.
+    iSplitL "Halive".
+    { iNext. unfold node_val_prop. iExists n'. iRight. iSplitR "Halive"; auto. }
+
     wp_pures.
+    wp_bind ( #node <- _ )%E.
+    iInv "Hnodeinv" as ">Hinv".
+    iDestruct "Hinv" as (n0) "[[H Halive] | [H Halive]]";
+    iDestruct "H" as %H'. inversion H'.
     wp_store.
-    iApply "HPost". 
+    iModIntro.
+
+    iSplitL "Halive".
+    iNext.
+    iExists (n'+1).
+    iRight; auto.
+
+    iDestruct "Hlkinv" as (n1) "Hγ1●".
+    iMod (ghost_var_update γ1 (n+1) with "Hγ1● Hγ1◯") as "[Hγ1● Hγ1◯]".
+    wp_pures.
+    iApply "HPost".
     iSplitL "Hγ1●".
     iExists (n+1); auto.
     iFrame; auto.
@@ -86,26 +120,38 @@ Section proof.
   Lemma update_node_none_spec : ∀ (n: Z) γ1 node,
       {{{
            node_lock_inv γ1
-           ∗ node_val_inv node n None γ1
+          ∗ node_val_inv node true γ1
+          ∗ node_own_inv node n γ1
     }}}
       update_node #node
     {{{ RET #0;
-          node_lock_inv γ1
-          ∗ (∃ n, node_val_inv node n None γ1)
+        node_lock_inv γ1
+        ∗ node_val_inv node true γ1
+        ∗ ∃ n, node_own_inv node n γ1
     }}}.
   Proof.
-    iIntros (n γ1 node Φ) "(Hlkinv & Hnodeinv) HPost".
+    iIntros (n γ1 node Φ) "(Hlkinv & #Hnodeinv & Hγ1◯) HPost".
     unfold node_val_inv.
-    iDestruct "Hnodeinv" as "([(H & Halive) | (H & Halive)] & Hown)";
-    iDestruct "H" as %H; inversion H. 
+    unfold node_val_prop.
     unfold update_node.
     unfold node_lock_inv.
-    iDestruct "Hlkinv" as (n') "Hlkinv".
+    unfold node_own_inv.
     wp_pures.
-    wp_load.
+
+    wp_bind ( ! #node )%E.
+    iInv "Hnodeinv" as ">Hinv".
+    iDestruct "Hinv" as (n') "[[H Halive] | [H Halive]]";
+    wp_load;
+    iDestruct "H" as %H; unfold not in H; simpl in H; try contradiction.
+    iModIntro.
+    iSplitL "Halive".
+    { iNext. unfold node_val_prop. iExists n'. iLeft. iSplitR "Halive"; auto. }
+
     wp_pures.
     iApply "HPost".
-    iSplitL "Hlkinv". iExists n'; auto.
-    unfold node_val_inv. iExists n. iFrame; auto. 
+    iDestruct "Hlkinv" as (n1) "Hγ1●".
+    iSplitL "Hγ1●".
+    iExists (n1); auto.
+    iFrame; auto.
   Qed.
 End proof.
